

\section*{5.1: A chemical process}
%%% AUTHOR: BENOIT SLUYSMANS %%%

In order to construct the state model, let's define the foowwing state variables:\\
\indent $x_1$ = species A concentration in the reactor\\
\indent $x_2$ = species B concentration in the reactor\\
\indent $x_3$ = species C concentration in the reactor\\
\indent $x_4$ = species B concentration in the recycling tank\\
\indent $V_1$ = reactor volume\\
\indent $V_2$ = recycling tank volume\\

By placing adequately the different flows $F_0, F_1, F_2, F_3, F_4$, it directly follows that
\begin{eqnarray*}
\dot{V_1} = F_1+F_2-F_0\\
\dot{V_2} = F_3+F_4-F_2
\end{eqnarray*}

By writing the system with two irreversible reactions, we obtain
\begin{eqnarray*}
A+B\rightarrow C \\
C\rightarrow A+B
\end{eqnarray*}

From there, we can write the stoechiometric matrix $C$ and, using the mass action law, the rate of these reactions $r_1$ and $r_2$:

\begin{equation*}
C = \begin{bmatrix}
-1 & 1\\
-1 & 1\\
1 & -1
\end{bmatrix}
\end{equation*}
and
\begin{eqnarray*}
r_1 &=& k_1 x_1 x_2\\
r_2 &=& k_2 x_3 
\end{eqnarray*}


If $x_A^{in}$ and $x_B^{in}$ are the concentrations of species A and B that enter the system, the balance equations give:
\begin{eqnarray*}
\dot{V_1x_1} &=& (-k_1 x_1 x_2+k_2 x_3 )V_1 + F_1 x_A^{in} - F_0 x_1 \\
\dot{V_1x_2} &=& (-k_1 x_1 x_2+k_2 x_3 )V_1 + F_2 x_4 - F_0 x_2 \\
\dot{V_1x_3} &=& (k_1 x_1 x_2-k_2 x_3 )V_1  - F_0 x_3 \\
\dot{V_2x_4} &=& F_0 x_2 + F_3 x_B^{in} - F_2 x_4
\end{eqnarray*}

As we have a perfect separator, it follows that $F_4 \rho_B = F_0 x_2$, with $\rho_B$ the density of species B. Finally, defining the input variables
\begin{eqnarray*}
u_0 &=& \frac{F_0}{V_1}\\
u_1 &=& \frac{F_1}{V_1}\\
u_2 &=& \frac{F_2}{V_1}\\
u_3 &=& \frac{F_3}{V_2}
\end{eqnarray*}
we obtain the following state model
\begin{eqnarray*}
\dot{x_1} &=& -k_1 x_1 x_2+k_2 x_3 + u_1 (x_A^{in}-x_1)-u_2 x_1\\
\dot{x_2} &=& -k_1 x_1 x_2+k_2 x_3 + u_2 x_4-(u_1+u_2)x_2\\
\dot{x_3} &=& k_1 x_1 x_2-k_2 x_3 -(u_1+u_2)x_3\\
\dot{x_4} &=& u_0\frac{V_1}{V_2}x_2(1-\frac{x_4}{\rho_B})+u_3(x_B^{in}-x_4)\\
\dot{V_1} &=& (u_1+u_2-u_0)V_1\\
\dot{V_2} &=& u_3V_2+(\frac{u_0x_2}{\rho_B}-u_2)V_1
\end{eqnarray*}






\section*{5.2: Reactors with separate power supplies}
%%% AUTHOR: BENOIT SLUYSMANS %%%

\subsection*{1.}
Let's define the input variables
\begin{eqnarray*}
u_1 &=& \frac{F_{01}}{V}\\
u_2 &=& \frac{F_{02}}{V}
\end{eqnarray*}
Remembering that the stoechiometric matrix was
\begin{eqnarray*}
C = \begin{bmatrix}
-1 & 0 \\
-1 & 0 \\
2 & -2 \\
0 & 1
\end{bmatrix}
\end{eqnarray*}
and that the rate of the two reactions were
\begin{eqnarray*}
r_1 &=& k_1x_1x_2e^{(-Kx_4)}\\
r_2 &=& k_2x_3^2
\end{eqnarray*}
we can write the following state model, with $c_1^{in}$ and $c_2^{in}$ the concentrations of species 1 and 2 that enter the system:
\begin{eqnarray*}
\dot{x_1} &=& -k_1x_1x_2e^{(-Kx_4)} + u_1 c_1^{in} - (u_1+u_2)x_1 \\
\dot{x_2} &=& -k_1x_1x_2e^{(-Kx_4)} + u_2 c_2^{in} - (u_1+u_2)x_2 \\
\dot{x_3} &=& 2k_1x_1x_2e^{(-Kx_4)} - 2k_2x_3^2 - (u_1+u_2)x_3 \\
\dot{x_4} &=& k_2x_3^2 - (u_1+u_2)x_4
\end{eqnarray*}
Indeed, the volume $V$ is constant and therefore $F_{out} = F_{01} + F_{02}$.

\subsection*{2.}
Here, $F_{01}+F_{02} = cst = dV \Leftrightarrow u_1 + u_2 = d$, so we only need one input variable. Let's take $u_1=w$ and $u_2=d-w$. We can rewrite
\begin{eqnarray*}
\dot{x_1} &=& -k_1x_1x_2e^{(-Kx_4)} + w c_1^{in} - d x_1 \\
\dot{x_2} &=& -k_1x_1x_2e^{(-Kx_4)} + (d-w) c_2^{in} - dx_2 \\
\dot{x_3} &=& 2k_1x_1x_2e^{(-Kx_4)} - 2k_2x_3^2 - dx_3 \\
\dot{x_4} &=& k_2x_3^2 - dx_4
\end{eqnarray*}
We can show that this model can be written as (5.8):
\begin{eqnarray*}
\frac{dx}{dt} &=& \begin{bmatrix}
-1 & 0 \\
-1 & 0 \\
2 & -2 \\
0 & 1
\end{bmatrix}
\begin{bmatrix}
k_1x_1x_2e^{(-Kx_4)} \\
k_2x_3^2
\end{bmatrix} - d\begin{bmatrix}
x_1\\
x_2\\
x_3\\
x_4
\end{bmatrix} + \begin{bmatrix}
w c_1^{in} \\
(d-w) c_2^{in}\\
0\\
0
\end{bmatrix}  \\
\Leftrightarrow \frac{dx}{dt} &=& C r(x) - q_{out}(x,w) + q_{in}(x,u)
\end{eqnarray*}




\section*{5.3: Gazeous reactives and products}

%%%%% AUTHOR: Florentin GOYENS %%%%%%%%%%%

We are working with the reactions of example 5.5:
\begin{eqnarray*}
X_1 + X_2 \rightarrow 2X_3 \\
X_3\rightarrow X_4.
\end{eqnarray*}
The velocities for the reactions are also given
$$r_{1}(x)=k_{1}x_{1}x_{2}e^{-Kx_{4}}$$
$$r_{2}(x)=k_{2}x_{3}^{2}.$$

According to the assumptions made, we compute the variation of each component over time. We account for the chemical reactions and the in/out flux.
$$\begin{array}{ccl}
\dot{x_{1}} & = & -1r_{1}(x)+\frac{F_{in}}{V}x_{1}^{in}-\frac{F_{out}}{V}x_{1}\\
\dot{x_{2}} & = & -1r_{1}(x)+a\frac{Q_{in}}{V}(x_{2}^{sat}-x_{2}) -\frac{F_{out}}{V}x_{2}\\
\dot{x_{3}} & = & 2r_{1}-2r_{2}-\frac{F_{out}}{V}x_{3}\\
\dot{x_{4}} & = & 1r_{2}-\frac{dx_{4}}{V}-\frac{F_{out}}{V}x_{4}
\end{array}$$

Assuming the volume constant gives $F_{in}=F_{out}$ and we set
$$\begin{array}{ccl}
u_{1} & = & \frac{F_{in}}{V}\\
u_{2} & = & \frac{Q_{in}}{V}.
\end{array}$$

Wich yields
$$\begin{array}{ccl}
\dot{x_{1}} & = & -1r_{1}(x)+u_{1}x_{1}^{in}-u_{1}x_{1}\\
\dot{x_{2}} & = & -1r_{1}(x)+au_{2}(x_{2}^{sat}-x_{2}) -u_{1}x_{2}\\
\dot{x_{3}} & = & 2r_{1}-2r_{2}-u_{1}x_{3}\\
\dot{x_{4}} & = & 1r_{2}-\frac{dx_{4}}{V}-u_{1}x_{4}.
\end{array}$$

This follows the standard form 
$$
\frac{dx}{dt}=
\underbrace{
\begin{pmatrix}
-1 & 0 \\
-1 & 0 \\
2 & -2 \\
0 & 1 \\
\end{pmatrix}}_{C} \underbrace{\begin{pmatrix}
k_{1}x_{1}x_{2}e^{-Kx_{4}}\\
k_{2}x_{3}^{2}\\
\end{pmatrix}}_{r(x)}-\underbrace{\begin{pmatrix}
u_{1}x_{1}\\
(u_{1}+au_{2})x_{2}\\
u_{1}x_{3}\\
(u_{1}+\frac{d}{V})x_{4}\\
\end{pmatrix}}_{q_{out}(x,u)}+
\underbrace{\begin{pmatrix}
u_{1}x_{1}^{in}\\
au_{2}x_{2}^{sat}\\
0\\
0\\
\end{pmatrix}}_{q_{in}(x,u)}.
$$




\section*{5.4: An aerobic biological wastewater treatment plant}

%% AUTHOR Florentin GOYENS

\textcolor{blue}{Il faudrait reprendre le schéma dans le correctif en français.}

The biotic reaction described in the first reactor can be summarized as follows
$$a_{1}O_{1}+a_{2}S_{1} \cata{X} a_{3}C_{1}+X_{1}$$

The microorganism X is a self-catalysor. We will follows Contois's model for a ecological system. Ence the velocity of the reaction is 
$$r(S_{1},O_{1},X_{1})=kX_{1}\dfrac{O_{1}}{O_{1}+K_{1}X_{1}}\dfrac{S_{1}}{S_{1}+K_{2}X_{1}}.$$
We will set $d$, the rate of mortality of the microorganisms. \textcolor{blue}{I think the corresponding term was missing in the equations of the french version.} 
The oxygen added apears at a rate of $\alpha Q_{in}(O_{sat}-O_{1})$. The volumes of all three reactors are assumed constant. We then express the mass balance of all the components
$$\begin{array}{ccl}
\dot{O_{1}} & = & \alpha Q_{in}(O_{sat}-O_{1})-a_{1}r-\dfrac{(F_{in}+F_{r})}{V_{1}}O_{1}+\dfrac{F_{in}}{V_{1}}O_{in}+\dfrac{F_{r}}{V_{1}}O_{3}\\
\dot{X_{1}} & = & r -dX_{1}-\dfrac{(F_{in}+F_{r})}{V_{1}}X_{1}+\dfrac{F_{r}}{V_{1}}X_{3}\\
\dot{S_{1}} & = & -a_{2}r+\dfrac{F_{in}}{V_{1}}S_{in}-\dfrac{F_{out}}{V_{1}}S_{1}\\
\dot{S_{2}} & = & \dfrac{F_{out}}{V_{2}}S_{1}-\dfrac{F_{out}}{V_{2}}S_{2}-\dfrac{F_{out}}{V_{2}}(S_{1}-S_{2})\\
\dot{O_{2}} & = & \dfrac{F_{out}}{V_{2}}(O_{1}-O_{2})\\
\dot{O_{3}} & = & \dfrac{F_{in}+F_{r}-F_{out}}{V_{2}}(O_{1}-O_{3})\\
\dot{X_{3}} & = & -\dfrac{F_{in}+F_{r}-F_{out}}{V_{3}}X_{3}+\dfrac{F_{in}+F_{r}}{V_{3}}X_{1}
\end{array}$$


This simplifies as 
$$\begin{pmatrix}
\dot{S_{1}}\\
\dot{O_{1}}\\
\dot{X_{1}}\\
\end{pmatrix}=\begin{pmatrix}
-a_{2}\\
-a_{1}\\
1\\
\end{pmatrix}
r(S_{1},O_{1},X_{1})+\dfrac{F_{in}}{V_{1}}\begin{pmatrix}
S_{in}-S_{1}\\
O_{in}-O_{1}\\
-X_{1}\\
\end{pmatrix}+
\dfrac{F_{r}}{V_{1}}
\begin{pmatrix}
-S_{1}\\
O_{3}-O_{1}\\
X_{3}-X_{1}\\
\end{pmatrix}+
\begin{pmatrix}
0\\
\alpha Q_{in}(O_{sat}-O_{1})\\
-dX_{1}\\
\end{pmatrix}$$
\begin{flushleft}

$$\begin{pmatrix}
\dot{S_{2}}\\
\dot{O_{2}}\\
\end{pmatrix}=
\dfrac{F_{in}}{V_{2}}\begin{pmatrix}
S_{1}-S_{2}\\
O_{1}-O_{2}\\
\end{pmatrix}$$
$$\begin{pmatrix}
\dot{O_{3}}\\
\dot{X_{3}}\\
\end{pmatrix}=
\dfrac{F_{in}+F_{r}-F_{out}}{V_{3}}\begin{pmatrix}
O_{1}-O_{3}\\
-X_{3}\\
\end{pmatrix}+
\dfrac{F_{in}+F_{r}}{V_{3}}
\begin{pmatrix}
O\\
X_{1}\\
\end{pmatrix}
$$




\section*{5.5: A nonconservative system}
%%% AUTHOR: BENOIT SLUYSMANS %%%
\subsection*{1.}
Starting from
\begin{eqnarray*}
X_1\rightarrow X_2+X_3 \\
X_3\rightarrow 2X_1+X_4
\end{eqnarray*}
we can write the stoechiometric matrix
\begin{eqnarray*}
\begin{bmatrix}
-1 & 2 \\
1 & 0 \\
1 & -1 \\
0 & 1
\end{bmatrix}
\end{eqnarray*}
and the rate of these reactions as described in the exercise
\begin{eqnarray*}
r_1 &=& k_1 x_1^2\\
r_2 &=& k_2 \frac{x_3}{K_3+x_3}\frac{K_2}{K_2+x_2}
\end{eqnarray*}
As this is a closed system, we can directly write the following state model
\begin{eqnarray*}
\dot{x_1} &=& - k_1 x_1^2 + 2k_2 \frac{x_3}{K_3+x_3}\frac{K_2}{K_2+x_2} \\
\dot{x_2} &=& k_1 x_1^2  \\
\dot{x_3} &=& k_1 x_1^2 - k_2 \frac{x_3}{K_3+x_3}\frac{K_2}{K_2+x_2} \\
\dot{x_4} &=& k_2 \frac{x_3}{K_3+x_3}\frac{K_2}{K_2+x_2}
\end{eqnarray*}


\subsection*{2.}
The system is conservative if $\exists w>0 | C^Tw = 0$, which is equivalent to
\begin{eqnarray*}
\begin{bmatrix}
-1 & 1 & 1 &0\\
2 & 0 & -1 & 1
\end{bmatrix}
\begin{bmatrix}
w_1 \\
w_2\\
w_3\\
w_4
\end{bmatrix} = \begin{bmatrix}
-w_1+w_2+w_3 \\
2w_1-w_3+w_4
\end{bmatrix} = \begin{bmatrix}
0 \\
0
\end{bmatrix}
\end{eqnarray*}
If we sum these two equations, we have $w_1+w_2+w_4=0$. That condition is impossible with $w_i > 0$. We can conclude that this system is nonconservative. Intuitively, we can see that one $X_1$ gives one $X_3$, and one $X_3$ gives two $X_1$, so the system would explode.

\subsection*{3.}
To make this system conservative, we can add a reactive to the first reaction, in order to modify $C$:
\begin{eqnarray*}
X_0 + X_1\rightarrow X_2+X_3 \\
X_3\rightarrow 2X_1+X_4
\end{eqnarray*}
\begin{eqnarray*}
C = \begin{bmatrix}
-1 & 0\\
-1 & 2 \\
1 & 0 \\
1 & -1 \\
0 & 1
\end{bmatrix}
\end{eqnarray*}
The condition to have a conservative system becomes 
\begin{eqnarray*}
\begin{bmatrix}
-1 & -1 & 1 & 1 &0\\
0 & 2 & 0 & -1 & 1
\end{bmatrix}
\begin{bmatrix}
w_1 \\
w_2\\
w_3\\
w_4\\
w_5
\end{bmatrix} = \begin{bmatrix}
-w_1-w_2+w_3+w_4 \\
2w_2-w_4+w_5
\end{bmatrix} = \begin{bmatrix}
0 \\
0
\end{bmatrix}
\end{eqnarray*}
which is verified if $w = (3,1,1,3,1)^T$. Here, the intuition is that we can produce two $X_1$ from one $X_1$ and another reactive $X_0$.

